tests/src/deref.rs
@@ -1,0 +1,30 @@
+//@ [!lean] skip
+
+use std::ops::Deref;
+use std::ops::DerefMut;
+
+pub fn use_deref_box<T>(x : &Box<T>) -> &T {
+    x.deref()
+}
+
+pub fn use_deref_mut_box<T>(x : &mut Box<T>) -> &mut T {
+    x.deref_mut()
+}
+
+pub fn test_deref_box() {
+    use std::ops::Deref;
+    use std::ops::DerefMut;
+    let mut b: Box<i32> = Box::new(0);
+    let x = b.deref_mut();
+    *x = 1;
+    let x = b.deref();
+    assert!(*x == 1);
+}
+
+pub fn use_deref_vec<T>(x : &Vec<T>) -> &[T] {
+    x.deref()
+}
+
+pub fn use_deref_mut_vec<T>(x : &mut Vec<T>) -> &mut [T] {
+    x.deref_mut()
+}
