tests/coq/misc/NoNestedBorrows.v
@@ -136,41 +136,28 @@ Definition test_list1 : result unit :=
 (** Unit test for [no_nested_borrows::test_list1] *)
 Check (test_list1)%return.
 
-(** [no_nested_borrows::test_box1]:
-    Source: 'tests/src/no_nested_borrows.rs', lines 129:0-137:1 *)
-Definition test_box1 : result unit :=
-  p <- alloc_boxed_Box_deref_mut 0%i32;
-  let (_, deref_mut_back) := p in
-  let b := deref_mut_back 1%i32 in
-  x <- alloc_boxed_Box_deref b;
-  massert (x s= 1%i32)
-.
-
-(** Unit test for [no_nested_borrows::test_box1] *)
-Check (test_box1)%return.
-
 (** [no_nested_borrows::copy_int]:
-    Source: 'tests/src/no_nested_borrows.rs', lines 139:0-141:1 *)
+    Source: 'tests/src/no_nested_borrows.rs', lines 128:0-130:1 *)
 Definition copy_int (x : i32) : result i32 :=
   Ok x.
 
 (** [no_nested_borrows::test_unreachable]:
-    Source: 'tests/src/no_nested_borrows.rs', lines 145:0-149:1 *)
+    Source: 'tests/src/no_nested_borrows.rs', lines 134:0-138:1 *)
 Definition test_unreachable (b : bool) : result unit :=
   massert b.
 
 (** [no_nested_borrows::test_panic]:
-    Source: 'tests/src/no_nested_borrows.rs', lines 152:0-156:1 *)
+    Source: 'tests/src/no_nested_borrows.rs', lines 141:0-145:1 *)
 Definition test_panic (b : bool) : result unit :=
   massert b.
 
 (** [no_nested_borrows::test_panic_msg]:
-    Source: 'tests/src/no_nested_borrows.rs', lines 160:0-164:1 *)
+    Source: 'tests/src/no_nested_borrows.rs', lines 149:0-153:1 *)
 Definition test_panic_msg (b : bool) : result unit :=
   massert b.
 
 (** [no_nested_borrows::test_copy_int]:
-    Source: 'tests/src/no_nested_borrows.rs', lines 167:0-172:1 *)
+    Source: 'tests/src/no_nested_borrows.rs', lines 156:0-161:1 *)
 Definition test_copy_int : result unit :=
   y <- copy_int 0%i32; massert (0%i32 s= y)
 .
@@ -179,13 +166,13 @@ Definition test_copy_int : result unit :=
 Check (test_copy_int)%return.
 
 (** [no_nested_borrows::is_cons]:
-    Source: 'tests/src/no_nested_borrows.rs', lines 174:0-179:1 *)
+    Source: 'tests/src/no_nested_borrows.rs', lines 163:0-168:1 *)
 Definition is_cons {T : Type} (l : List_t T) : result bool :=
   match l with | List_Cons _ _ => Ok true | List_Nil => Ok false end
 .
 
 (** [no_nested_borrows::test_is_cons]:
-    Source: 'tests/src/no_nested_borrows.rs', lines 181:0-185:1 *)
+    Source: 'tests/src/no_nested_borrows.rs', lines 170:0-174:1 *)
 Definition test_is_cons : result unit :=
   b <- is_cons (List_Cons 0%i32 List_Nil); massert b
 .
@@ -194,13 +181,13 @@ Definition test_is_cons : result unit :=
 Check (test_is_cons)%return.
 
 (** [no_nested_borrows::split_list]:
-    Source: 'tests/src/no_nested_borrows.rs', lines 187:0-192:1 *)
+    Source: 'tests/src/no_nested_borrows.rs', lines 176:0-181:1 *)
 Definition split_list {T : Type} (l : List_t T) : result (T * (List_t T)) :=
   match l with | List_Cons hd tl => Ok (hd, tl) | List_Nil => Fail_ Failure end
 .
 
 (** [no_nested_borrows::test_split_list]:
-    Source: 'tests/src/no_nested_borrows.rs', lines 195:0-200:1 *)
+    Source: 'tests/src/no_nested_borrows.rs', lines 184:0-189:1 *)
 Definition test_split_list : result unit :=
   p <- split_list (List_Cons 0%i32 List_Nil);
   let (hd, _) := p in
@@ -211,7 +198,7 @@ Definition test_split_list : result unit :=
 Check (test_split_list)%return.
 
 (** [no_nested_borrows::choose]:
-    Source: 'tests/src/no_nested_borrows.rs', lines 202:0-208:1 *)
+    Source: 'tests/src/no_nested_borrows.rs', lines 191:0-197:1 *)
 Definition choose
   {T : Type} (b : bool) (x : T) (y : T) : result (T * (T -> (T * T))) :=
   if b
@@ -220,7 +207,7 @@ Definition choose
 .
 
 (** [no_nested_borrows::choose_test]:
-    Source: 'tests/src/no_nested_borrows.rs', lines 210:0-219:1 *)
+    Source: 'tests/src/no_nested_borrows.rs', lines 199:0-208:1 *)
 Definition choose_test : result unit :=
   p <- choose true 0%i32 0%i32;
   let (z, choose_back) := p in
@@ -235,23 +222,23 @@ Definition choose_test : result unit :=
 Check (choose_test)%return.
 
 (** [no_nested_borrows::test_char]:
-    Source: 'tests/src/no_nested_borrows.rs', lines 222:0-224:1 *)
+    Source: 'tests/src/no_nested_borrows.rs', lines 211:0-213:1 *)
 Definition test_char : result char :=
   Ok (char_of_byte Coq.Init.Byte.x61).
 
 (** [no_nested_borrows::panic_mut_borrow]:
-    Source: 'tests/src/no_nested_borrows.rs', lines 227:0-229:1 *)
+    Source: 'tests/src/no_nested_borrows.rs', lines 216:0-218:1 *)
 Definition panic_mut_borrow (i : u32) : result u32 :=
   Fail_ Failure.
 
 (** [no_nested_borrows::Tree]
-    Source: 'tests/src/no_nested_borrows.rs', lines 232:0-235:1 *)
+    Source: 'tests/src/no_nested_borrows.rs', lines 221:0-224:1 *)
 Inductive Tree_t (T : Type) :=
 | Tree_Leaf : T -> Tree_t T
 | Tree_Node : T -> NodeElem_t T -> Tree_t T -> Tree_t T
 
 (** [no_nested_borrows::NodeElem]
-    Source: 'tests/src/no_nested_borrows.rs', lines 237:0-240:1 *)
+    Source: 'tests/src/no_nested_borrows.rs', lines 226:0-229:1 *)
 with NodeElem_t (T : Type) :=
 | NodeElem_Cons : Tree_t T -> NodeElem_t T -> NodeElem_t T
 | NodeElem_Nil : NodeElem_t T
@@ -264,7 +251,7 @@ Arguments NodeElem_Cons { _ }.
 Arguments NodeElem_Nil { _ }.
 
 (** [no_nested_borrows::list_length]:
-    Source: 'tests/src/no_nested_borrows.rs', lines 272:0-277:1 *)
+    Source: 'tests/src/no_nested_borrows.rs', lines 261:0-266:1 *)
 Fixpoint list_length {T : Type} (l : List_t T) : result u32 :=
   match l with
   | List_Cons _ l1 => i <- list_length l1; u32_add 1%u32 i
@@ -273,7 +260,7 @@ Fixpoint list_length {T : Type} (l : List_t T) : result u32 :=
 .
 
 (** [no_nested_borrows::list_nth_shared]:
-    Source: 'tests/src/no_nested_borrows.rs', lines 280:0-293:1 *)
+    Source: 'tests/src/no_nested_borrows.rs', lines 269:0-282:1 *)
 Fixpoint list_nth_shared {T : Type} (l : List_t T) (i : u32) : result T :=
   match l with
   | List_Cons x tl =>
@@ -283,7 +270,7 @@ Fixpoint list_nth_shared {T : Type} (l : List_t T) (i : u32) : result T :=
 .
 
 (** [no_nested_borrows::list_nth_mut]:
-    Source: 'tests/src/no_nested_borrows.rs', lines 296:0-309:1 *)
+    Source: 'tests/src/no_nested_borrows.rs', lines 285:0-298:1 *)
 Fixpoint list_nth_mut
   {T : Type} (l : List_t T) (i : u32) : result (T * (T -> List_t T)) :=
   match l with
@@ -302,7 +289,7 @@ Fixpoint list_nth_mut
 .
 
 (** [no_nested_borrows::list_rev_aux]:
-    Source: 'tests/src/no_nested_borrows.rs', lines 312:0-322:1 *)
+    Source: 'tests/src/no_nested_borrows.rs', lines 301:0-311:1 *)
 Fixpoint list_rev_aux
   {T : Type} (li : List_t T) (lo : List_t T) : result (List_t T) :=
   match li with
@@ -312,13 +299,13 @@ Fixpoint list_rev_aux
 .
 
 (** [no_nested_borrows::list_rev]:
-    Source: 'tests/src/no_nested_borrows.rs', lines 326:0-329:1 *)
+    Source: 'tests/src/no_nested_borrows.rs', lines 315:0-318:1 *)
 Definition list_rev {T : Type} (l : List_t T) : result (List_t T) :=
   let (li, _) := core_mem_replace l List_Nil in list_rev_aux li List_Nil
 .
 
 (** [no_nested_borrows::test_list_functions]:
-    Source: 'tests/src/no_nested_borrows.rs', lines 331:0-345:1 *)
+    Source: 'tests/src/no_nested_borrows.rs', lines 320:0-334:1 *)
 Definition test_list_functions : result unit :=
   let l := List_Cons 2%i32 List_Nil in
   let l1 := List_Cons 1%i32 l in
@@ -345,7 +332,7 @@ Definition test_list_functions : result unit :=
 Check (test_list_functions)%return.
 
 (** [no_nested_borrows::id_mut_pair1]:
-    Source: 'tests/src/no_nested_borrows.rs', lines 347:0-349:1 *)
+    Source: 'tests/src/no_nested_borrows.rs', lines 336:0-338:1 *)
 Definition id_mut_pair1
   {T1 : Type} {T2 : Type} (x : T1) (y : T2) :
   result ((T1 * T2) * ((T1 * T2) -> (T1 * T2)))
@@ -354,7 +341,7 @@ Definition id_mut_pair1
 .
 
 (** [no_nested_borrows::id_mut_pair2]:
-    Source: 'tests/src/no_nested_borrows.rs', lines 351:0-353:1 *)
+    Source: 'tests/src/no_nested_borrows.rs', lines 340:0-342:1 *)
 Definition id_mut_pair2
   {T1 : Type} {T2 : Type} (p : (T1 * T2)) :
   result ((T1 * T2) * ((T1 * T2) -> (T1 * T2)))
@@ -363,7 +350,7 @@ Definition id_mut_pair2
 .
 
 (** [no_nested_borrows::id_mut_pair3]:
-    Source: 'tests/src/no_nested_borrows.rs', lines 355:0-357:1 *)
+    Source: 'tests/src/no_nested_borrows.rs', lines 344:0-346:1 *)
 Definition id_mut_pair3
   {T1 : Type} {T2 : Type} (x : T1) (y : T2) :
   result ((T1 * T2) * (T1 -> T1) * (T2 -> T2))
@@ -372,7 +359,7 @@ Definition id_mut_pair3
 .
 
 (** [no_nested_borrows::id_mut_pair4]:
-    Source: 'tests/src/no_nested_borrows.rs', lines 359:0-361:1 *)
+    Source: 'tests/src/no_nested_borrows.rs', lines 348:0-350:1 *)
 Definition id_mut_pair4
   {T1 : Type} {T2 : Type} (p : (T1 * T2)) :
   result ((T1 * T2) * (T1 -> T1) * (T2 -> T2))
@@ -381,7 +368,7 @@ Definition id_mut_pair4
 .
 
 (** [no_nested_borrows::StructWithTuple]
-    Source: 'tests/src/no_nested_borrows.rs', lines 366:0-368:1 *)
+    Source: 'tests/src/no_nested_borrows.rs', lines 355:0-357:1 *)
 Record StructWithTuple_t (T1 : Type) (T2 : Type) :=
 mkStructWithTuple_t {
   structWithTuple_p : (T1 * T2);
@@ -392,25 +379,25 @@ Arguments mkStructWithTuple_t { _ } { _ }.
 Arguments structWithTuple_p { _ } { _ }.
 
 (** [no_nested_borrows::new_tuple1]:
-    Source: 'tests/src/no_nested_borrows.rs', lines 370:0-372:1 *)
+    Source: 'tests/src/no_nested_borrows.rs', lines 359:0-361:1 *)
 Definition new_tuple1 : result (StructWithTuple_t u32 u32) :=
   Ok {| structWithTuple_p := (1%u32, 2%u32) |}
 .
 
 (** [no_nested_borrows::new_tuple2]:
-    Source: 'tests/src/no_nested_borrows.rs', lines 374:0-376:1 *)
+    Source: 'tests/src/no_nested_borrows.rs', lines 363:0-365:1 *)
 Definition new_tuple2 : result (StructWithTuple_t i16 i16) :=
   Ok {| structWithTuple_p := (1%i16, 2%i16) |}
 .
 
 (** [no_nested_borrows::new_tuple3]:
-    Source: 'tests/src/no_nested_borrows.rs', lines 378:0-380:1 *)
+    Source: 'tests/src/no_nested_borrows.rs', lines 367:0-369:1 *)
 Definition new_tuple3 : result (StructWithTuple_t u64 i64) :=
   Ok {| structWithTuple_p := (1%u64, 2%i64) |}
 .
 
 (** [no_nested_borrows::StructWithPair]
-    Source: 'tests/src/no_nested_borrows.rs', lines 383:0-385:1 *)
+    Source: 'tests/src/no_nested_borrows.rs', lines 372:0-374:1 *)
 Record StructWithPair_t (T1 : Type) (T2 : Type) :=
 mkStructWithPair_t {
   structWithPair_p : Pair_t T1 T2;
@@ -421,13 +408,13 @@ Arguments mkStructWithPair_t { _ } { _ }.
 Arguments structWithPair_p { _ } { _ }.
 
 (** [no_nested_borrows::new_pair1]:
-    Source: 'tests/src/no_nested_borrows.rs', lines 387:0-393:1 *)
+    Source: 'tests/src/no_nested_borrows.rs', lines 376:0-382:1 *)
 Definition new_pair1 : result (StructWithPair_t u32 u32) :=
   Ok {| structWithPair_p := {| pair_x := 1%u32; pair_y := 2%u32 |} |}
 .
 
 (** [no_nested_borrows::test_constants]:
-    Source: 'tests/src/no_nested_borrows.rs', lines 395:0-400:1 *)
+    Source: 'tests/src/no_nested_borrows.rs', lines 384:0-389:1 *)
 Definition test_constants : result unit :=
   swt <- new_tuple1;
   let (i, _) := swt.(structWithTuple_p) in
@@ -446,7 +433,7 @@ Definition test_constants : result unit :=
 Check (test_constants)%return.
 
 (** [no_nested_borrows::test_weird_borrows1]:
-    Source: 'tests/src/no_nested_borrows.rs', lines 404:0-412:1 *)
+    Source: 'tests/src/no_nested_borrows.rs', lines 393:0-401:1 *)
 Definition test_weird_borrows1 : result unit :=
   Ok tt.
 
@@ -454,7 +441,7 @@ Definition test_weird_borrows1 : result unit :=
 Check (test_weird_borrows1)%return.
 
 (** [no_nested_borrows::test_mem_replace]:
-    Source: 'tests/src/no_nested_borrows.rs', lines 414:0-418:1 *)
+    Source: 'tests/src/no_nested_borrows.rs', lines 403:0-407:1 *)
 Definition test_mem_replace (px : u32) : result u32 :=
   let (y, _) := core_mem_replace px 1%u32 in
   _ <- massert (y s= 0%u32);
@@ -462,110 +449,110 @@ Definition test_mem_replace (px : u32) : result u32 :=
 .
 
 (** [no_nested_borrows::test_shared_borrow_bool1]:
-    Source: 'tests/src/no_nested_borrows.rs', lines 421:0-430:1 *)
+    Source: 'tests/src/no_nested_borrows.rs', lines 410:0-419:1 *)
 Definition test_shared_borrow_bool1 (b : bool) : result u32 :=
   if b then Ok 0%u32 else Ok 1%u32
 .
 
 (** [no_nested_borrows::test_shared_borrow_bool2]:
-    Source: 'tests/src/no_nested_borrows.rs', lines 434:0-444:1 *)
+    Source: 'tests/src/no_nested_borrows.rs', lines 423:0-433:1 *)
 Definition test_shared_borrow_bool2 : result u32 :=
   Ok 0%u32.
 
 (** [no_nested_borrows::test_shared_borrow_enum1]:
-    Source: 'tests/src/no_nested_borrows.rs', lines 449:0-457:1 *)
+    Source: 'tests/src/no_nested_borrows.rs', lines 438:0-446:1 *)
 Definition test_shared_borrow_enum1 (l : List_t u32) : result u32 :=
   match l with | List_Cons _ _ => Ok 1%u32 | List_Nil => Ok 0%u32 end
 .
 
 (** [no_nested_borrows::test_shared_borrow_enum2]:
-    Source: 'tests/src/no_nested_borrows.rs', lines 461:0-470:1 *)
+    Source: 'tests/src/no_nested_borrows.rs', lines 450:0-459:1 *)
 Definition test_shared_borrow_enum2 : result u32 :=
   Ok 0%u32.
 
 (** [no_nested_borrows::incr]:
-    Source: 'tests/src/no_nested_borrows.rs', lines 472:0-474:1 *)
+    Source: 'tests/src/no_nested_borrows.rs', lines 461:0-463:1 *)
 Definition incr (x : u32) : result u32 :=
   u32_add x 1%u32.
 
 (** [no_nested_borrows::call_incr]:
-    Source: 'tests/src/no_nested_borrows.rs', lines 476:0-479:1 *)
+    Source: 'tests/src/no_nested_borrows.rs', lines 465:0-468:1 *)
 Definition call_incr (x : u32) : result u32 :=
   incr x.
 
 (** [no_nested_borrows::read_then_incr]:
-    Source: 'tests/src/no_nested_borrows.rs', lines 481:0-485:1 *)
+    Source: 'tests/src/no_nested_borrows.rs', lines 470:0-474:1 *)
 Definition read_then_incr (x : u32) : result (u32 * u32) :=
   x1 <- u32_add x 1%u32; Ok (x, x1)
 .
 
 (** [no_nested_borrows::Tuple]
-    Source: 'tests/src/no_nested_borrows.rs', lines 487:0-487:33 *)
+    Source: 'tests/src/no_nested_borrows.rs', lines 476:0-476:33 *)
 Definition Tuple_t (T1 : Type) (T2 : Type) : Type := T1 * T2.
 
 (** [no_nested_borrows::read_tuple]:
-    Source: 'tests/src/no_nested_borrows.rs', lines 489:0-491:1 *)
+    Source: 'tests/src/no_nested_borrows.rs', lines 478:0-480:1 *)
 Definition read_tuple (x : (u32 * u32)) : result u32 :=
   let (i, _) := x in Ok i
 .
 
 (** [no_nested_borrows::update_tuple]:
-    Source: 'tests/src/no_nested_borrows.rs', lines 493:0-495:1 *)
+    Source: 'tests/src/no_nested_borrows.rs', lines 482:0-484:1 *)
 Definition update_tuple (x : (u32 * u32)) : result (u32 * u32) :=
   let (_, i) := x in Ok (1%u32, i)
 .
 
 (** [no_nested_borrows::read_tuple_struct]:
-    Source: 'tests/src/no_nested_borrows.rs', lines 497:0-499:1 *)
+    Source: 'tests/src/no_nested_borrows.rs', lines 486:0-488:1 *)
 Definition read_tuple_struct (x : Tuple_t u32 u32) : result u32 :=
   let (i, _) := x in Ok i
 .
 
 (** [no_nested_borrows::update_tuple_struct]:
-    Source: 'tests/src/no_nested_borrows.rs', lines 501:0-503:1 *)
+    Source: 'tests/src/no_nested_borrows.rs', lines 490:0-492:1 *)
 Definition update_tuple_struct
   (x : Tuple_t u32 u32) : result (Tuple_t u32 u32) :=
   let (_, i) := x in Ok (1%u32, i)
 .
 
 (** [no_nested_borrows::create_tuple_struct]:
-    Source: 'tests/src/no_nested_borrows.rs', lines 505:0-507:1 *)
+    Source: 'tests/src/no_nested_borrows.rs', lines 494:0-496:1 *)
 Definition create_tuple_struct
   (x : u32) (y : u64) : result (Tuple_t u32 u64) :=
   Ok (x, y)
 .
 
 (** [no_nested_borrows::IdType]
-    Source: 'tests/src/no_nested_borrows.rs', lines 510:0-510:24 *)
+    Source: 'tests/src/no_nested_borrows.rs', lines 499:0-499:24 *)
 Definition IdType_t (T : Type) : Type := T.
 
 (** [no_nested_borrows::use_id_type]:
-    Source: 'tests/src/no_nested_borrows.rs', lines 512:0-514:1 *)
+    Source: 'tests/src/no_nested_borrows.rs', lines 501:0-503:1 *)
 Definition use_id_type {T : Type} (x : IdType_t T) : result T :=
   Ok x.
 
 (** [no_nested_borrows::create_id_type]:
-    Source: 'tests/src/no_nested_borrows.rs', lines 516:0-518:1 *)
+    Source: 'tests/src/no_nested_borrows.rs', lines 505:0-507:1 *)
 Definition create_id_type {T : Type} (x : T) : result (IdType_t T) :=
   Ok x.
 
 (** [no_nested_borrows::not_bool]:
-    Source: 'tests/src/no_nested_borrows.rs', lines 520:0-522:1 *)
+    Source: 'tests/src/no_nested_borrows.rs', lines 509:0-511:1 *)
 Definition not_bool (x : bool) : result bool :=
   Ok (negb x).
 
 (** [no_nested_borrows::not_u32]:
-    Source: 'tests/src/no_nested_borrows.rs', lines 524:0-526:1 *)
+    Source: 'tests/src/no_nested_borrows.rs', lines 513:0-515:1 *)
 Definition not_u32 (x : u32) : result u32 :=
   Ok (scalar_not x).
 
 (** [no_nested_borrows::not_i32]:
-    Source: 'tests/src/no_nested_borrows.rs', lines 528:0-530:1 *)
+    Source: 'tests/src/no_nested_borrows.rs', lines 517:0-519:1 *)
 Definition not_i32 (x : i32) : result i32 :=
   Ok (scalar_not x).
 
 (** [no_nested_borrows::borrow_mut_tuple]:
-    Source: 'tests/src/no_nested_borrows.rs', lines 532:0-534:1 *)
+    Source: 'tests/src/no_nested_borrows.rs', lines 521:0-523:1 *)
 Definition borrow_mut_tuple
   {T : Type} {U : Type} (x : (T * U)) :
   result ((T * U) * ((T * U) -> (T * U)))
@@ -574,18 +561,18 @@ Definition borrow_mut_tuple
 .
 
 (** [no_nested_borrows::ExpandSimpliy::Wrapper]
-    Source: 'tests/src/no_nested_borrows.rs', lines 538:4-538:32 *)
+    Source: 'tests/src/no_nested_borrows.rs', lines 527:4-527:32 *)
 Definition ExpandSimpliy_Wrapper_t (T : Type) : Type := T * T.
 
 (** [no_nested_borrows::ExpandSimpliy::check_expand_simplify_symb1]:
-    Source: 'tests/src/no_nested_borrows.rs', lines 540:4-546:5 *)
+    Source: 'tests/src/no_nested_borrows.rs', lines 529:4-535:5 *)
 Definition expandSimpliy_check_expand_simplify_symb1
   (x : ExpandSimpliy_Wrapper_t bool) : result (ExpandSimpliy_Wrapper_t bool) :=
   let (b, _) := x in if b then Ok x else Ok x
 .
 
 (** [no_nested_borrows::ExpandSimpliy::Wrapper2]
-    Source: 'tests/src/no_nested_borrows.rs', lines 548:4-551:5 *)
+    Source: 'tests/src/no_nested_borrows.rs', lines 537:4-540:5 *)
 Record ExpandSimpliy_Wrapper2_t :=
 mkExpandSimpliy_Wrapper2_t {
   expandSimpliy_Wrapper2_b : bool; expandSimpliy_Wrapper2_x : u32;
@@ -593,7 +580,7 @@ mkExpandSimpliy_Wrapper2_t {
 .
 
 (** [no_nested_borrows::ExpandSimpliy::check_expand_simplify_symb2]:
-    Source: 'tests/src/no_nested_borrows.rs', lines 553:4-559:5 *)
+    Source: 'tests/src/no_nested_borrows.rs', lines 542:4-548:5 *)
 Definition expandSimpliy_check_expand_simplify_symb2
   (x : ExpandSimpliy_Wrapper2_t) : result ExpandSimpliy_Wrapper2_t :=
   if x.(expandSimpliy_Wrapper2_b)
