tests/lean/NoNestedBorrows.lean
@@ -128,40 +128,28 @@ def test_list1 : Result Unit :=
 /- Unit test for [no_nested_borrows::test_list1] -/
 #assert (test_list1 == ok ())
 
-/- [no_nested_borrows::test_box1]:
-   Source: 'tests/src/no_nested_borrows.rs', lines 129:0-137:1 -/
-def test_box1 : Result Unit :=
-  do
-  let (_, deref_mut_back) ← alloc.boxed.Box.deref_mut 0#i32
-  let b := deref_mut_back 1#i32
-  let x ← alloc.boxed.Box.deref b
-  massert (x = 1#i32)
-
-/- Unit test for [no_nested_borrows::test_box1] -/
-#assert (test_box1 == ok ())
-
 /- [no_nested_borrows::copy_int]:
-   Source: 'tests/src/no_nested_borrows.rs', lines 139:0-141:1 -/
+   Source: 'tests/src/no_nested_borrows.rs', lines 128:0-130:1 -/
 def copy_int (x : I32) : Result I32 :=
   ok x
 
 /- [no_nested_borrows::test_unreachable]:
-   Source: 'tests/src/no_nested_borrows.rs', lines 145:0-149:1 -/
+   Source: 'tests/src/no_nested_borrows.rs', lines 134:0-138:1 -/
 def test_unreachable (b : Bool) : Result Unit :=
   massert b
 
 /- [no_nested_borrows::test_panic]:
-   Source: 'tests/src/no_nested_borrows.rs', lines 152:0-156:1 -/
+   Source: 'tests/src/no_nested_borrows.rs', lines 141:0-145:1 -/
 def test_panic (b : Bool) : Result Unit :=
   massert b
 
 /- [no_nested_borrows::test_panic_msg]:
-   Source: 'tests/src/no_nested_borrows.rs', lines 160:0-164:1 -/
+   Source: 'tests/src/no_nested_borrows.rs', lines 149:0-153:1 -/
 def test_panic_msg (b : Bool) : Result Unit :=
   massert b
 
 /- [no_nested_borrows::test_copy_int]:
-   Source: 'tests/src/no_nested_borrows.rs', lines 167:0-172:1 -/
+   Source: 'tests/src/no_nested_borrows.rs', lines 156:0-161:1 -/
 def test_copy_int : Result Unit :=
   do
   let y ← copy_int 0#i32
@@ -171,14 +159,14 @@ def test_copy_int : Result Unit :=
 #assert (test_copy_int == ok ())
 
 /- [no_nested_borrows::is_cons]:
-   Source: 'tests/src/no_nested_borrows.rs', lines 174:0-179:1 -/
+   Source: 'tests/src/no_nested_borrows.rs', lines 163:0-168:1 -/
 def is_cons {T : Type} (l : List T) : Result Bool :=
   match l with
   | List.Cons _ _ => ok true
   | List.Nil => ok false
 
 /- [no_nested_borrows::test_is_cons]:
-   Source: 'tests/src/no_nested_borrows.rs', lines 181:0-185:1 -/
+   Source: 'tests/src/no_nested_borrows.rs', lines 170:0-174:1 -/
 def test_is_cons : Result Unit :=
   do
   let b ← is_cons (List.Cons 0#i32 List.Nil)
@@ -188,14 +176,14 @@ def test_is_cons : Result Unit :=
 #assert (test_is_cons == ok ())
 
 /- [no_nested_borrows::split_list]:
-   Source: 'tests/src/no_nested_borrows.rs', lines 187:0-192:1 -/
+   Source: 'tests/src/no_nested_borrows.rs', lines 176:0-181:1 -/
 def split_list {T : Type} (l : List T) : Result (T × (List T)) :=
   match l with
   | List.Cons hd tl => ok (hd, tl)
   | List.Nil => fail panic
 
 /- [no_nested_borrows::test_split_list]:
-   Source: 'tests/src/no_nested_borrows.rs', lines 195:0-200:1 -/
+   Source: 'tests/src/no_nested_borrows.rs', lines 184:0-189:1 -/
 def test_split_list : Result Unit :=
   do
   let (hd, _) ← split_list (List.Cons 0#i32 List.Nil)
@@ -205,7 +193,7 @@ def test_split_list : Result Unit :=
 #assert (test_split_list == ok ())
 
 /- [no_nested_borrows::choose]:
-   Source: 'tests/src/no_nested_borrows.rs', lines 202:0-208:1 -/
+   Source: 'tests/src/no_nested_borrows.rs', lines 191:0-197:1 -/
 def choose
   {T : Type} (b : Bool) (x : T) (y : T) : Result (T × (T → (T × T))) :=
   if b
@@ -215,7 +203,7 @@ def choose
        ok (y, back)
 
 /- [no_nested_borrows::choose_test]:
-   Source: 'tests/src/no_nested_borrows.rs', lines 210:0-219:1 -/
+   Source: 'tests/src/no_nested_borrows.rs', lines 199:0-208:1 -/
 def choose_test : Result Unit :=
   do
   let (z, choose_back) ← choose true 0#i32 0#i32
@@ -229,25 +217,25 @@ def choose_test : Result Unit :=
 #assert (choose_test == ok ())
 
 /- [no_nested_borrows::test_char]:
-   Source: 'tests/src/no_nested_borrows.rs', lines 222:0-224:1 -/
+   Source: 'tests/src/no_nested_borrows.rs', lines 211:0-213:1 -/
 def test_char : Result Char :=
   ok 'a'
 
 /- [no_nested_borrows::panic_mut_borrow]:
-   Source: 'tests/src/no_nested_borrows.rs', lines 227:0-229:1 -/
+   Source: 'tests/src/no_nested_borrows.rs', lines 216:0-218:1 -/
 def panic_mut_borrow (i : U32) : Result U32 :=
   fail panic
 
 mutual
 
 /- [no_nested_borrows::Tree]
-   Source: 'tests/src/no_nested_borrows.rs', lines 232:0-235:1 -/
+   Source: 'tests/src/no_nested_borrows.rs', lines 221:0-224:1 -/
 inductive Tree (T : Type) where
 | Leaf : T → Tree T
 | Node : T → NodeElem T → Tree T → Tree T
 
 /- [no_nested_borrows::NodeElem]
-   Source: 'tests/src/no_nested_borrows.rs', lines 237:0-240:1 -/
+   Source: 'tests/src/no_nested_borrows.rs', lines 226:0-229:1 -/
 inductive NodeElem (T : Type) where
 | Cons : Tree T → NodeElem T → NodeElem T
 | Nil : NodeElem T
@@ -255,7 +243,7 @@ inductive NodeElem (T : Type) where
 end
 
 /- [no_nested_borrows::list_length]:
-   Source: 'tests/src/no_nested_borrows.rs', lines 272:0-277:1 -/
+   Source: 'tests/src/no_nested_borrows.rs', lines 261:0-266:1 -/
 divergent def list_length {T : Type} (l : List T) : Result U32 :=
   match l with
   | List.Cons _ l1 => do
@@ -264,7 +252,7 @@ divergent def list_length {T : Type} (l : List T) : Result U32 :=
   | List.Nil => ok 0#u32
 
 /- [no_nested_borrows::list_nth_shared]:
-   Source: 'tests/src/no_nested_borrows.rs', lines 280:0-293:1 -/
+   Source: 'tests/src/no_nested_borrows.rs', lines 269:0-282:1 -/
 divergent def list_nth_shared {T : Type} (l : List T) (i : U32) : Result T :=
   match l with
   | List.Cons x tl =>
@@ -276,7 +264,7 @@ divergent def list_nth_shared {T : Type} (l : List T) (i : U32) : Result T :=
   | List.Nil => fail panic
 
 /- [no_nested_borrows::list_nth_mut]:
-   Source: 'tests/src/no_nested_borrows.rs', lines 296:0-309:1 -/
+   Source: 'tests/src/no_nested_borrows.rs', lines 285:0-298:1 -/
 divergent def list_nth_mut
   {T : Type} (l : List T) (i : U32) : Result (T × (T → List T)) :=
   match l with
@@ -294,7 +282,7 @@ divergent def list_nth_mut
   | List.Nil => fail panic
 
 /- [no_nested_borrows::list_rev_aux]:
-   Source: 'tests/src/no_nested_borrows.rs', lines 312:0-322:1 -/
+   Source: 'tests/src/no_nested_borrows.rs', lines 301:0-311:1 -/
 divergent def list_rev_aux
   {T : Type} (li : List T) (lo : List T) : Result (List T) :=
   match li with
@@ -302,13 +290,13 @@ divergent def list_rev_aux
   | List.Nil => ok lo
 
 /- [no_nested_borrows::list_rev]:
-   Source: 'tests/src/no_nested_borrows.rs', lines 326:0-329:1 -/
+   Source: 'tests/src/no_nested_borrows.rs', lines 315:0-318:1 -/
 def list_rev {T : Type} (l : List T) : Result (List T) :=
   let (li, _) := core.mem.replace l List.Nil
   list_rev_aux li List.Nil
 
 /- [no_nested_borrows::test_list_functions]:
-   Source: 'tests/src/no_nested_borrows.rs', lines 331:0-345:1 -/
+   Source: 'tests/src/no_nested_borrows.rs', lines 320:0-334:1 -/
 def test_list_functions : Result Unit :=
   do
   let l := List.Cons 2#i32 List.Nil
@@ -334,7 +322,7 @@ def test_list_functions : Result Unit :=
 #assert (test_list_functions == ok ())
 
 /- [no_nested_borrows::id_mut_pair1]:
-   Source: 'tests/src/no_nested_borrows.rs', lines 347:0-349:1 -/
+   Source: 'tests/src/no_nested_borrows.rs', lines 336:0-338:1 -/
 def id_mut_pair1
   {T1 : Type} {T2 : Type} (x : T1) (y : T2) :
   Result ((T1 × T2) × ((T1 × T2) → (T1 × T2)))
@@ -342,7 +330,7 @@ def id_mut_pair1
   ok ((x, y), fun ret => ret)
 
 /- [no_nested_borrows::id_mut_pair2]:
-   Source: 'tests/src/no_nested_borrows.rs', lines 351:0-353:1 -/
+   Source: 'tests/src/no_nested_borrows.rs', lines 340:0-342:1 -/
 def id_mut_pair2
   {T1 : Type} {T2 : Type} (p : (T1 × T2)) :
   Result ((T1 × T2) × ((T1 × T2) → (T1 × T2)))
@@ -350,7 +338,7 @@ def id_mut_pair2
   ok (p, fun ret => ret)
 
 /- [no_nested_borrows::id_mut_pair3]:
-   Source: 'tests/src/no_nested_borrows.rs', lines 355:0-357:1 -/
+   Source: 'tests/src/no_nested_borrows.rs', lines 344:0-346:1 -/
 def id_mut_pair3
   {T1 : Type} {T2 : Type} (x : T1) (y : T2) :
   Result ((T1 × T2) × (T1 → T1) × (T2 → T2))
@@ -358,7 +346,7 @@ def id_mut_pair3
   ok ((x, y), fun ret => ret, fun ret => ret)
 
 /- [no_nested_borrows::id_mut_pair4]:
-   Source: 'tests/src/no_nested_borrows.rs', lines 359:0-361:1 -/
+   Source: 'tests/src/no_nested_borrows.rs', lines 348:0-350:1 -/
 def id_mut_pair4
   {T1 : Type} {T2 : Type} (p : (T1 × T2)) :
   Result ((T1 × T2) × (T1 → T1) × (T2 → T2))
@@ -366,37 +354,37 @@ def id_mut_pair4
   ok (p, fun ret => ret, fun ret => ret)
 
 /- [no_nested_borrows::StructWithTuple]
-   Source: 'tests/src/no_nested_borrows.rs', lines 366:0-368:1 -/
+   Source: 'tests/src/no_nested_borrows.rs', lines 355:0-357:1 -/
 structure StructWithTuple (T1 : Type) (T2 : Type) where
   p : (T1 × T2)
 
 /- [no_nested_borrows::new_tuple1]:
-   Source: 'tests/src/no_nested_borrows.rs', lines 370:0-372:1 -/
+   Source: 'tests/src/no_nested_borrows.rs', lines 359:0-361:1 -/
 def new_tuple1 : Result (StructWithTuple U32 U32) :=
   ok { p := (1#u32, 2#u32) }
 
 /- [no_nested_borrows::new_tuple2]:
-   Source: 'tests/src/no_nested_borrows.rs', lines 374:0-376:1 -/
+   Source: 'tests/src/no_nested_borrows.rs', lines 363:0-365:1 -/
 def new_tuple2 : Result (StructWithTuple I16 I16) :=
   ok { p := (1#i16, 2#i16) }
 
 /- [no_nested_borrows::new_tuple3]:
-   Source: 'tests/src/no_nested_borrows.rs', lines 378:0-380:1 -/
+   Source: 'tests/src/no_nested_borrows.rs', lines 367:0-369:1 -/
 def new_tuple3 : Result (StructWithTuple U64 I64) :=
   ok { p := (1#u64, 2#i64) }
 
 /- [no_nested_borrows::StructWithPair]
-   Source: 'tests/src/no_nested_borrows.rs', lines 383:0-385:1 -/
+   Source: 'tests/src/no_nested_borrows.rs', lines 372:0-374:1 -/
 structure StructWithPair (T1 : Type) (T2 : Type) where
   p : Pair T1 T2
 
 /- [no_nested_borrows::new_pair1]:
-   Source: 'tests/src/no_nested_borrows.rs', lines 387:0-393:1 -/
+   Source: 'tests/src/no_nested_borrows.rs', lines 376:0-382:1 -/
 def new_pair1 : Result (StructWithPair U32 U32) :=
   ok { p := { x := 1#u32, y := 2#u32 } }
 
 /- [no_nested_borrows::test_constants]:
-   Source: 'tests/src/no_nested_borrows.rs', lines 395:0-400:1 -/
+   Source: 'tests/src/no_nested_borrows.rs', lines 384:0-389:1 -/
 def test_constants : Result Unit :=
   do
   let swt ← new_tuple1
@@ -415,7 +403,7 @@ def test_constants : Result Unit :=
 #assert (test_constants == ok ())
 
 /- [no_nested_borrows::test_weird_borrows1]:
-   Source: 'tests/src/no_nested_borrows.rs', lines 404:0-412:1 -/
+   Source: 'tests/src/no_nested_borrows.rs', lines 393:0-401:1 -/
 def test_weird_borrows1 : Result Unit :=
   ok ()
 
@@ -423,7 +411,7 @@ def test_weird_borrows1 : Result Unit :=
 #assert (test_weird_borrows1 == ok ())
 
 /- [no_nested_borrows::test_mem_replace]:
-   Source: 'tests/src/no_nested_borrows.rs', lines 414:0-418:1 -/
+   Source: 'tests/src/no_nested_borrows.rs', lines 403:0-407:1 -/
 def test_mem_replace (px : U32) : Result U32 :=
   do
   let (y, _) := core.mem.replace px 1#u32
@@ -431,110 +419,110 @@ def test_mem_replace (px : U32) : Result U32 :=
   ok 2#u32
 
 /- [no_nested_borrows::test_shared_borrow_bool1]:
-   Source: 'tests/src/no_nested_borrows.rs', lines 421:0-430:1 -/
+   Source: 'tests/src/no_nested_borrows.rs', lines 410:0-419:1 -/
 def test_shared_borrow_bool1 (b : Bool) : Result U32 :=
   if b
   then ok 0#u32
   else ok 1#u32
 
 /- [no_nested_borrows::test_shared_borrow_bool2]:
-   Source: 'tests/src/no_nested_borrows.rs', lines 434:0-444:1 -/
+   Source: 'tests/src/no_nested_borrows.rs', lines 423:0-433:1 -/
 def test_shared_borrow_bool2 : Result U32 :=
   ok 0#u32
 
 /- [no_nested_borrows::test_shared_borrow_enum1]:
-   Source: 'tests/src/no_nested_borrows.rs', lines 449:0-457:1 -/
+   Source: 'tests/src/no_nested_borrows.rs', lines 438:0-446:1 -/
 def test_shared_borrow_enum1 (l : List U32) : Result U32 :=
   match l with
   | List.Cons _ _ => ok 1#u32
   | List.Nil => ok 0#u32
 
 /- [no_nested_borrows::test_shared_borrow_enum2]:
-   Source: 'tests/src/no_nested_borrows.rs', lines 461:0-470:1 -/
+   Source: 'tests/src/no_nested_borrows.rs', lines 450:0-459:1 -/
 def test_shared_borrow_enum2 : Result U32 :=
   ok 0#u32
 
 /- [no_nested_borrows::incr]:
-   Source: 'tests/src/no_nested_borrows.rs', lines 472:0-474:1 -/
+   Source: 'tests/src/no_nested_borrows.rs', lines 461:0-463:1 -/
 def incr (x : U32) : Result U32 :=
   x + 1#u32
 
 /- [no_nested_borrows::call_incr]:
-   Source: 'tests/src/no_nested_borrows.rs', lines 476:0-479:1 -/
+   Source: 'tests/src/no_nested_borrows.rs', lines 465:0-468:1 -/
 def call_incr (x : U32) : Result U32 :=
   incr x
 
 /- [no_nested_borrows::read_then_incr]:
-   Source: 'tests/src/no_nested_borrows.rs', lines 481:0-485:1 -/
+   Source: 'tests/src/no_nested_borrows.rs', lines 470:0-474:1 -/
 def read_then_incr (x : U32) : Result (U32 × U32) :=
   do
   let x1 ← x + 1#u32
   ok (x, x1)
 
 /- [no_nested_borrows::Tuple]
-   Source: 'tests/src/no_nested_borrows.rs', lines 487:0-487:33 -/
+   Source: 'tests/src/no_nested_borrows.rs', lines 476:0-476:33 -/
 def Tuple (T1 : Type) (T2 : Type) := T1 × T2
 
 /- [no_nested_borrows::read_tuple]:
-   Source: 'tests/src/no_nested_borrows.rs', lines 489:0-491:1 -/
+   Source: 'tests/src/no_nested_borrows.rs', lines 478:0-480:1 -/
 def read_tuple (x : (U32 × U32)) : Result U32 :=
   let (i, _) := x
   ok i
 
 /- [no_nested_borrows::update_tuple]:
-   Source: 'tests/src/no_nested_borrows.rs', lines 493:0-495:1 -/
+   Source: 'tests/src/no_nested_borrows.rs', lines 482:0-484:1 -/
 def update_tuple (x : (U32 × U32)) : Result (U32 × U32) :=
   let (_, i) := x
   ok (1#u32, i)
 
 /- [no_nested_borrows::read_tuple_struct]:
-   Source: 'tests/src/no_nested_borrows.rs', lines 497:0-499:1 -/
+   Source: 'tests/src/no_nested_borrows.rs', lines 486:0-488:1 -/
 def read_tuple_struct (x : Tuple U32 U32) : Result U32 :=
   let (i, _) := x
   ok i
 
 /- [no_nested_borrows::update_tuple_struct]:
-   Source: 'tests/src/no_nested_borrows.rs', lines 501:0-503:1 -/
+   Source: 'tests/src/no_nested_borrows.rs', lines 490:0-492:1 -/
 def update_tuple_struct (x : Tuple U32 U32) : Result (Tuple U32 U32) :=
   let (_, i) := x
   ok (1#u32, i)
 
 /- [no_nested_borrows::create_tuple_struct]:
-   Source: 'tests/src/no_nested_borrows.rs', lines 505:0-507:1 -/
+   Source: 'tests/src/no_nested_borrows.rs', lines 494:0-496:1 -/
 def create_tuple_struct (x : U32) (y : U64) : Result (Tuple U32 U64) :=
   ok (x, y)
 
 /- [no_nested_borrows::IdType]
-   Source: 'tests/src/no_nested_borrows.rs', lines 510:0-510:24 -/
+   Source: 'tests/src/no_nested_borrows.rs', lines 499:0-499:24 -/
 @[reducible] def IdType (T : Type) := T
 
 /- [no_nested_borrows::use_id_type]:
-   Source: 'tests/src/no_nested_borrows.rs', lines 512:0-514:1 -/
+   Source: 'tests/src/no_nested_borrows.rs', lines 501:0-503:1 -/
 def use_id_type {T : Type} (x : IdType T) : Result T :=
   ok x
 
 /- [no_nested_borrows::create_id_type]:
-   Source: 'tests/src/no_nested_borrows.rs', lines 516:0-518:1 -/
+   Source: 'tests/src/no_nested_borrows.rs', lines 505:0-507:1 -/
 def create_id_type {T : Type} (x : T) : Result (IdType T) :=
   ok x
 
 /- [no_nested_borrows::not_bool]:
-   Source: 'tests/src/no_nested_borrows.rs', lines 520:0-522:1 -/
+   Source: 'tests/src/no_nested_borrows.rs', lines 509:0-511:1 -/
 def not_bool (x : Bool) : Result Bool :=
   ok (¬ x)
 
 /- [no_nested_borrows::not_u32]:
-   Source: 'tests/src/no_nested_borrows.rs', lines 524:0-526:1 -/
+   Source: 'tests/src/no_nested_borrows.rs', lines 513:0-515:1 -/
 def not_u32 (x : U32) : Result U32 :=
   ok (~~~ x)
 
 /- [no_nested_borrows::not_i32]:
-   Source: 'tests/src/no_nested_borrows.rs', lines 528:0-530:1 -/
+   Source: 'tests/src/no_nested_borrows.rs', lines 517:0-519:1 -/
 def not_i32 (x : I32) : Result I32 :=
   ok (~~~ x)
 
 /- [no_nested_borrows::borrow_mut_tuple]:
-   Source: 'tests/src/no_nested_borrows.rs', lines 532:0-534:1 -/
+   Source: 'tests/src/no_nested_borrows.rs', lines 521:0-523:1 -/
 def borrow_mut_tuple
   {T : Type} {U : Type} (x : (T × U)) :
   Result ((T × U) × ((T × U) → (T × U)))
@@ -542,11 +530,11 @@ def borrow_mut_tuple
   ok (x, fun ret => ret)
 
 /- [no_nested_borrows::ExpandSimpliy::Wrapper]
-   Source: 'tests/src/no_nested_borrows.rs', lines 538:4-538:32 -/
+   Source: 'tests/src/no_nested_borrows.rs', lines 527:4-527:32 -/
 def ExpandSimpliy.Wrapper (T : Type) := T × T
 
 /- [no_nested_borrows::ExpandSimpliy::check_expand_simplify_symb1]:
-   Source: 'tests/src/no_nested_borrows.rs', lines 540:4-546:5 -/
+   Source: 'tests/src/no_nested_borrows.rs', lines 529:4-535:5 -/
 def ExpandSimpliy.check_expand_simplify_symb1
   (x : ExpandSimpliy.Wrapper Bool) : Result (ExpandSimpliy.Wrapper Bool) :=
   let (b, _) := x
@@ -555,13 +543,13 @@ def ExpandSimpliy.check_expand_simplify_symb1
   else ok x
 
 /- [no_nested_borrows::ExpandSimpliy::Wrapper2]
-   Source: 'tests/src/no_nested_borrows.rs', lines 548:4-551:5 -/
+   Source: 'tests/src/no_nested_borrows.rs', lines 537:4-540:5 -/
 structure ExpandSimpliy.Wrapper2 where
   b : Bool
   x : U32
 
 /- [no_nested_borrows::ExpandSimpliy::check_expand_simplify_symb2]:
-   Source: 'tests/src/no_nested_borrows.rs', lines 553:4-559:5 -/
+   Source: 'tests/src/no_nested_borrows.rs', lines 542:4-548:5 -/
 def ExpandSimpliy.check_expand_simplify_symb2
   (x : ExpandSimpliy.Wrapper2) : Result ExpandSimpliy.Wrapper2 :=
   if x.b
